before tracking error "Bound term variable not found (after unmangling): f#99067"

examples/algorithms/Uf.fst
@@ -7,44 +7,34 @@ open FStar.Classical
 open FStar.Ghost
 open FStar.ST
 open FStar.TSet
+open FStar.FunctionalExtensionality
 
+
+(** TODO : Prove that forall u1 u2 : ufh a h. u1.parent = u2.parent ==> u1 = u2  using reification *)
 
 type uf (a : Type) : Type = { content:a ; parent:ref (option (uf a)) }
 
-noeq type reachable (#a:eqtype) (h:heap) (x:uf a) : uf a -> Type =
-| Immediately : y:(uf a){sel h y.parent = Some x} -> reachable h x y
-| Later : y:(uf a) -> reachable h x y -> z:(uf a){sel h z.parent = Some y} -> reachable h x z
-
-(*
-val give_witness : #p:Type -> p -> Pure unit (requires True) (ensures (fun _ -> p))
-let give_witness #p x = give_proof (return_squash x)
-
-val intro_impl : #p:Type -> #q:Type -> f:(p -> Tot q) -> Tot (p ==> q)
-let intro_impl #p #q f =
-  let g : p -> GTot q = f in
-  return_squash g
-
-val intro_forall : #a:Type -> #p:(a -> Type) -> $f:(x:a -> Tot (p x)) -> Tot (forall x. p x)
-let intro_forall #a #p f =
-  let g : x:a -> GTot (p x) = f in
-  return_squash g
-
-val give_proof0 : #p:Type0 -> p -> Pure unit (requires True) (ensures (fun _ -> p))
-let give_proof0 #p _ = ()
-*)
 
 noeq type funcaccessible (#a:Type0) (f: a -> GTot (option a)) (u : a) : Type0 =
 | FAcc : next:(match f u with | Some v -> funcaccessible f v | None -> unit) -> funcaccessible f u
 
 
 let ufh a h = x:(uf a){Heap.contains h x.parent}
-let state_true (h:heap) = True
 
 let reach (a:eqtype) h (u : uf a) : GTot (option (uf a)) = sel h u.parent
 
-assume val recall_step : #a:eqtype -> h:heap -> z:uf a -> y:uf a -> Lemma (requires (sel h z.parent = Some y)) (ensures (Heap.contains h y.parent))
+assume val recall_step : #a:eqtype -> h:heap -> z:uf a -> y:uf a -> Lemma (requires (reach a h z = Some y)) (ensures (Heap.contains h y.parent))
 
 
+let reprfun (a:eqtype) (h:heap) = f:(uf a -> GTot (uf a)){
+  (forall u. if Heap.contains h u.parent then Heap.contains h (f u).parent else u = f u) /\
+  (forall (u:ufh a h). sel h (f u).parent = None /\(sel h u.parent = None ==> f u = u)) /\
+  (forall (u:ufh a h) (v:ufh a h). sel h u.parent = Some v ==> f u = f v)
+}
+
+
+
+(*
 let rec recall_reachable (#a:eqtype) (h:heap) (u1:uf a) (u2:uf a) (w:reachable h u1 u2) : Lemma (requires (Heap.contains h u2.parent)) (ensures (Heap.contains h u1.parent)) (decreases w) =
   match w with
   | Immediately z -> recall_step h z u1
@@ -61,25 +51,69 @@ let rec pushforward_reachable (#a:eqtype) (h0:heap) (h1:heap) (u1:uf a) (u2: uf 
     match w with
     | Immediately z -> Immediately z
     | Later y w0 z -> recall_step h0 z y ; Later y (pushforward_reachable h0 h1 u1 y w0) z
+*)
 
 //assume val recall_reachable : #a:eqtype -> h:heap -> u1:(uf a) -> u2:(uf a) -> Lemma (Heap.contains h u1.parent /\ reachable h u2 u1 ==> Heap.contains h u2.parent)
 //assume val pullback_reachable : #a:eqtype -> h0:heap -> h1:heap -> u1:(uf a) -> u2:(uf a) -> reachable h1 u1 u2 -> Pure (reachable h0 u1 u2) (requires (modifies_none h0 h1 /\ Heap.contains h0 u2.parent)) (ensures (fun _ -> True))
 
 
-let uf_invariant (a:eqtype) (h:heap) : Type0 = (forall (u0:ufh a h). funcaccessible (reach a h) u0) ///\ (forall (u0: ufh a h) (u1: ufh a h). u0.parent = u1.parent ==> u0 = u1) // * (u1: uf a -> reachable h u1 u0 -> Lemma (u1.parent <> u0.parent)))
+let uf_invariant (a:eqtype) (h:heap) : Type0 = (forall (u0:ufh a h). funcaccessible (reach a h) u0)
 let uf_invariant_fun (#a:eqtype) (h:heap) : Tot Type0 = (u0:ufh a h) -> GTot (funcaccessible (reach a h) u0)
 
-let maintain_uf_invariant (a:eqtype) (h0:heap) (h1:heap) ($f : uf_invariant_fun h0 -> GTot (uf_invariant_fun h1)) : Lemma (requires (uf_invariant a h0)) (ensures (uf_invariant a h1)) =
+let maintain_uf_invariant (#a:eqtype) (#h0:heap) (#h1:heap) ($f : uf_invariant_fun h0 -> GTot (uf_invariant_fun h1)) : Lemma (requires (uf_invariant a h0)) (ensures (uf_invariant a h1)) =
   give_proof #(uf_invariant a h1) (map_squash (get_proof (uf_invariant a h0)) (fun (sq_uf_inv0 : squash (uf_invariant_fun h0)) -> map_squash sq_uf_inv0 f))
 
 assume val uf_invariant_termination : (a:eqtype) -> (h:heap) -> (u:ufh a h) -> (p:ufh a h) -> Lemma (requires (uf_invariant a h /\ sel h u.parent = Some p)) (ensures (p << u))
 
-//let typeof (a:Type) ($f : a) = f
+
+(** Ghost functional extensionality **)
+type gfun (a:Type) (b:Type) = a -> GTot b
+
+type gfeq (#a:Type) (#b:Type) (f:gfun a b) (g:gfun a b) =
+    (forall x.{:pattern (f x) \/ (g x)} f x == g x)
+
+assume GhostExtensionality : forall (a:Type) (b:Type) (f: gfun a b) (g: gfun a b).
+                        {:pattern gfeq #a #b f g} gfeq #a #b f g <==> f==g
 
 
-//assume val axiom1_dep2 : #a:Type -> #b:(a->Type) -> #c:(x:a -> y:b x -> Type) -> f:(x:a -> y:b x -> Tot (c x y)) -> x:a -> y: b x -> Lemma (f x y << f)
+let reprfun_prop (#a:eqtype) (h:heap) (f1:reprfun a h) (f2:reprfun a h) : Lemma (requires (uf_invariant a h)) (ensures (f1 == f2)) =
+  let w = get_proof (uf_invariant a h) in (* TODO : check that not having this proposition in the closire of equality_proof is normal *)
+  let rec equality_proof (u:ufh a h) : Lemma (requires True) (ensures (f1 u == f2 u)) (decreases u) =
+    match sel h u.parent with
+    | None -> ()
+    | Some v -> recall_step h u v ; give_proof w ; uf_invariant_termination a h u v ; equality_proof v
+  in
+  forall_intro equality_proof ; assert (gfeq f1 f2)
 
-//let pullback_contains (#a:Type) (h0:heap) (h1:heap) (x:ref a) (r0:ref a) : Lemma (requires (exists v. h1 == upd h0 r0 v /\ Heap.contains h1 x /\ x <> r0)) (ensures (Heap.contains h0 x)) = ()
+
+let retrieve_reprfun (a:eqtype) (h:heap) : Pure (reprfun a h) (requires (uf_invariant a h)) (ensures (fun _ -> True)) =
+  let w = get_proof (uf_invariant a h) in
+  let rec f (u:uf a) : Ghost (uf a) (requires True) (ensures (fun r -> if Heap.contains h u.parent then Heap.contains h r.parent /\ sel h r.parent = None /\ (sel h u.parent = None ==> u = r) else u = r)) =
+    if Heap.contains h u.parent then
+      match reach a h u with | None -> u | Some v -> recall_step h u v ; give_proof w ; uf_invariant_termination a h u v ; f v
+    else u
+  in
+  //assert (forall u. sel h (f u).parent = None /\ (sel h u.parent = None ==> f u = u)) ;
+  let f : uf a -> GTot (uf a) = f in
+  let rec reprfun_prop (u:ufh a h) (v:ufh a h) : Lemma (requires (reach a h u = Some v)) (ensures (f u == f v)) = admit ()
+    (*match reach a h v with
+    | None -> ()
+    | Some w -> recall_step h v w ; reprfun_prop v w *)
+  in (*TODO : investigate why it does not go through *)
+  let reprfun_prop' (u:ufh a h) : Lemma (forall (v:ufh a h). sel h u.parent = Some v ==> f u = f v) = forall_intro (move_requires (reprfun_prop u)) in
+  forall_intro reprfun_prop' ;
+  //assert (forall (u:ufh a h) (v:ufh a h). sel h u.parent = Some v ==> f u = f v) ;
+  f
+
+
+let same_reprfun (a:eqtype) (h0:heap) (h1:heap) : Pure Type0 (requires (uf_invariant a h0 /\ uf_invariant a h1)) (ensures (fun _ -> True)) =
+  let f0 = retrieve_reprfun a h0 in let f1 = retrieve_reprfun a h1 in f1 == f0
+
+let merge_reprfun (a:eqtype) (h0:heap) (h1:heap) (x:uf a) (y:uf a) (z:uf a) : Pure Type0 (requires (uf_invariant a h0 /\ uf_invariant a h1)) (ensures (fun _ -> True)) =
+  let f0 = retrieve_reprfun a h0 in
+  let f1 = retrieve_reprfun a h1 in
+  f1 == (fun w -> if f0 w = f0 x || f0 w = f0 y then z else f0 w)
+
 
 (* Without invariants :
    let make_uf (#a:eqtype) (x:a) : St (uf a) =
@@ -87,7 +121,7 @@ assume val uf_invariant_termination : (a:eqtype) -> (h:heap) -> (u:ufh a h) -> (
 *)
 
 
-let make_uf (#a:eqtype) (x:a) : ST (uf a) (requires (uf_invariant a)) (ensures (fun h0 x h1 -> modifies_none h0 h1 /\ uf_invariant a h1)) =
+let make_uf (#a:eqtype) (x:a) : ST (uf a) (requires (uf_invariant a)) (ensures (fun h0 x h1 -> modifies_none h0 h1 /\ uf_invariant a h1 /\ uf_invariant a h0 /\ same_reprfun a h0 h1)) =
   let h0 = get () in
   let res : uf a = { content = x ; parent = alloc None } in
   let h1 = get () in
@@ -95,38 +129,13 @@ let make_uf (#a:eqtype) (x:a) : ST (uf a) (requires (uf_invariant a)) (ensures (
     let rec pushforward_accessible (u:ufh a h1) (acc0 : funcaccessible (reach a h0) u) : GTot (funcaccessible (reach a h1) u) (decreases acc0) =
       match reach a h1 u with | None -> FAcc () | Some v -> recall_step h1 u v ; FAcc (pushforward_accessible v acc0.next)
     in if u.parent = res.parent then FAcc () else let u : uf a = u in pushforward_accessible u (uf_inv0 u)
-  in maintain_uf_invariant a h0 h1 uf_inv1 ;
+  in maintain_uf_invariant uf_inv1 ;
   res
 
 
 
-(*
-let intro_forall_impl (#a:Type) (#b:a -> Type0) (#c:a -> Type0) ($f:x:a -> b x -> Lemma (c x)) : Lemma (forall (x:a). b x ==> c x) =
-  let f0 (x:a) (y:b x) : GTot (squash (c x)) = f x y ; get_proof (c x) in
-  let f1 (x:a) : GTot (squash (squash (b x -> GTot (c x)))) = return_squash (squash_double_arrow (return_squash (f0 x))) in
-  let f2 : squash (x:a -> GTot (squash (b x -> GTot (c x)))) = squash_double_arrow (return_squash f1) in
-  let f3 : squash (x:a -> GTot (b x ==> c x)) = f2 in
-  let res : (forall (x:a). b x ==> c x) = f3 in
-  give_witness res
-  *)
-
-(*
-let rec collect_above (#a:eqtype) (h:heap) (u : ufh a h) : Ghost (set aref) (requires (uf_invariant a h)) (ensures (fun s -> forall v. (sel h v.parent <> None /\ (v = u \/ reachable h v u)) <==> mem (Ref v.parent) s)) (decreases u) =
-  match sel h u.parent with
-    | None ->
-      let f (v:uf a) : GTot ((reachable h v u) ==> False) = impl_intro_gtot (let g (w:reachable h v u) : GTot False = match w with in g) in
-      give_witness (forall_intro_gtot f) ;
-      assert (forall v. ~(reachable h v u)) ;
-      empty
-    | Some p ->
-      let f (v:uf a) (w:reachable h v u): Lemma (v.parent = p.parent \/ reachable h v p) = match w with | Immediately _ -> () | Later _ w0 _ -> give_witness w0 in
-      forall_intro (let g (v:uf a) : Lemma (reachable h v u ==> v.parent = p.parent \/ reachable h v p) = impl_intro (f v) in g) ;
-      assert(forall (v:uf a). (reachable h v u ==> (v.parent = p.parent \/ reachable h v p)))  ;
-      recall_step h u p ; uf_invariant_termination a h u p ; admit () ; singleton (Ref u.parent) `union` collect_above h p
-*)
-
-
 let distinct_cell_lemma (#a:eqtype) (h:heap) (r1:ref a) (r2: ref a) : Lemma (sel h r1 <> sel h r2 ==> r1 <> r2) = ()
+
 
 (* Without invariants :
 
@@ -135,13 +144,14 @@ let distinct_cell_lemma (#a:eqtype) (h:heap) (r1:ref a) (r2: ref a) : Lemma (sel
     | none -> u
     | some p ->
       let r = root p in
-      u.parent := r 
+      u.parent := r
       r
 *)
 
-let rec root (#a:eqtype) (u:uf a) : ST (uf a) (requires (uf_invariant a)) (ensures (fun h0 r h1 -> (* Heap.contains h0 u.parent /\ uf_invariant a h0 /\ modifies (collect_above h0 u) h0 h1 /\*) uf_invariant a h1 /\ (r = u \/ reachable h0 r u) /\ sel h0 r.parent = None /\ sel h1 r.parent = None)) (decreases u) (* WARNING : check the decrease clause by hand for now *) =
+(** TODO : why do I need to ask for uf_invariant a h0 in the post-condition ??? *)
+let rec root (#a:eqtype) (u:uf a) : ST (uf a) (requires (uf_invariant a)) (ensures (fun h0 r h1 -> uf_invariant a h0 /\ uf_invariant a h1 /\ same_reprfun a h0 h1 /\ (*sel h0 r.parent = None /\ sel h1 r.parent = None*) retrieve_reprfun a h1 u = r) ) (decreases u) (* WARNING : check the decrease clause by hand for now *) =
   match !u.parent with
-  | None -> admit () ; u
+  | None -> u
   | Some p ->
     let h0 = get () in
     recall u.parent ;
@@ -150,51 +160,24 @@ let rec root (#a:eqtype) (u:uf a) : ST (uf a) (requires (uf_invariant a)) (ensur
     assert ( p << u ) ;
     let r = root p in
     let h1 = get () in
-    assert (sel h0 u.parent = Some p) ;
+//   assert (sel h0 u.parent = Some p) ;
     distinct_cell_lemma h0 r.parent u.parent ;
-    assert (r.parent <> u.parent) ;
+//    assert (r.parent <> u.parent) ;
     recall u.parent ;
     u.parent := Some r ;
     let h2 = get () in
-    assert (forall (u0 : ufh a h2). Heap.contains h1 u0.parent);
-    assert (forall (u0 : ufh a h2). u0.parent <> u.parent ==> reach a h2 u0 = reach a h1 u0);
+//    assert (forall (u0 : ufh a h2). Heap.contains h1 u0.parent);
+//    assert (forall (u0 : ufh a h2). u0.parent <> u.parent ==> reach a h2 u0 = reach a h1 u0);
     let uf_inv2 (uf_inv1: uf_invariant_fun h1) (u1:ufh a h2) : GTot (funcaccessible (reach a h2) u1) =
       let rec pushforward (u0:ufh a h1) (w : funcaccessible (reach a h1) u0) : GTot (funcaccessible (reach a h2) u0) (decreases w) =
         if u0.parent = u.parent
-        then ( match reach a h2 u0 with | Some r0 -> let wr0 : funcaccessible (reach a h2) r0 = match reach a h2 r0 with | None -> FAcc () in FAcc wr0 ) (* TODO : Something's wrong here FAcc (FAcc ()) should be enough  *)
+        then begin match reach a h2 u0 with
+          | Some r0 -> let wr0 : funcaccessible (reach a h2) r0 = match reach a h2 r0 with | None -> FAcc () in FAcc wr0
+          end(* TODO : Something's wrong here FAcc (FAcc ()) should be enough  *)
         else match reach a h2 u0 with | None -> FAcc () | Some v -> recall_step h1 u0 v ; FAcc (pushforward v w.next)
       in let u1 : uf a = u1 in pushforward u1 (uf_inv1 u1)
-    in maintain_uf_invariant a h1 h2 uf_inv2 ;
-    assert (uf_invariant a h2) ;
-    if p = r then give_witness #(reachable h0 r u) (Immediately u) else give_proof (map_squash (get_proof (reachable h0 r p)) (fun w -> Later p w u)) ;
-    assert (reachable h0 r u) ;
-    //admit () ;
-    (*let sqw0 : squash (reachable h0 r u) =
-      let res = if r = p then return_squash (Immediately p u) else map_squash (get_proof (reachable h0 r p)) (fun w -> Later r p w u) in
-      admit () ; res
-    in
-    give_proof (bind_squash sqw0 (fun w0 -> bind_squash (get_proof (uf_invariant a h0)) (fun uf_inv0 -> (snd (uf_inv0 u)) r w0 ; get_proof (r.parent <> u.parent)))) ;
-    assert (u.parent <> r.parent) ;
-    assert (u <> r) ;
-    assert (sel h1 r.parent = None) ;
-    let aux (uf_inv: uf_invariant a h1) : GTot (squash (uf_invariant a h2)) =
-      let wf (u1:ufh a h2) : GTot (funcaccessible (reach a h2) u1) =
-        let root_accessible : funcaccessible (reach a h2) r = FAcc () in
-        let u_accessible : funcaccessible (reach a h2) u = FAcc (root_accessible) in
-        let rec pushforward (u0:uf a) (w : funcaccessible (reach a h1) u0) : GTot (funcaccessible (reach a h2) u0) (decreases w) =
-          if u0 = u then u_accessible else match reach a h2 u0 with | None -> FAcc () | Some v -> FAcc (pushforward w.next)
-        in
-        pushforward u1 (fst (uf_inv u1))
-      in
-      let antialiasing (u1:ufh a h2) (u0:uf a) (w:reachable h2 u0 u1) : Lemma (u1.parent <> u0.parent) = admit ()
-      (* idea : transform a "reachable h2 u0 u1" to a "rechable h0 u0 u1" by using the existing "reachable h0 r u0" whenever we stumble on a element in "collect_above h0 u (...)" *)
-      (* then apply the uf_invariant for h0 to this rechability proof *)
-      in
-      return_squash begin fun u0 -> (wf u0, antialiasing u0) end
-    in
-    give_proof (bind_squash (get_proof (uf_invariant a h1)) aux) ;
-   assert (uf_invariant a h2) ;
-  assert (sel h2 r.parent = None) ;*)
+    in maintain_uf_invariant uf_inv2 ;
+//   if p = r then give_witness #(reachable h0 r u) (Immediately u) else give_proof (map_squash (get_proof (reachable h0 r p)) (fun w -> Later p w u)) ;
     r
 
 
@@ -206,27 +189,13 @@ let rec root (#a:eqtype) (u:uf a) : ST (uf a) (requires (uf_invariant a)) (ensur
 
 
 
-let rec uf_equiv (#a:eqtype) (u1:uf a) (u2:uf a) : ST bool (requires (uf_invariant a)) (ensures (fun h0 _ h1 -> modifies ((collect_above h0 u1 (admit ())) `union` (collect_above h0 u2 (admit ()))) h0 h1 /\ uf_invariant a h1)) =
+let rec uf_equiv (#a:eqtype) (u1:uf a) (u2:uf a) : ST bool (requires (uf_invariant a)) (ensures (fun h0 _ h1 -> uf_invariant a h1)) =
   let h0 = get () in
   let r1 = root u1 in
   let h1 = get () in
   let r2 = root u2 in
   let h2 = get () in
-  admit () ;
   r1 = r2
-
-
-
-
-
-
-  let rec collect_all_above (#a:eqtype) (h:heap) (u : uf a) (w:funcaccessible (reach a h) u) : Ghost (set aref) (requires True) (ensures (fun s -> forall v. (v.parent = u.parent \/ reachable h v u) <==> mem (Ref v.parent) s)) (decreases w) =
-    match sel h u.parent with
-      | None -> let f (v:uf a) : Tot ((reachable h v u) ==> False) = intro_impl (fun w -> match w with) in give_witness (intro_forall f) ; assert (forall v. ~(reachable h v u)) ; singleton (Ref u.parent)
-      | Some p ->
-        let f (v:uf a) (w:reachable h v u): Lemma (v.parent = p.parent \/ reachable h v p) = match w with | Immediately _ _ -> () | Later _ _ w0 _ -> give_witness w0 in
-        intro_forall_impl f ; assert(forall (v:uf a). (reachable h v u ==> (v.parent = p.parent \/ reachable h v p)))  ;
-        recall_step h u p ; admit () ; singleton (Ref u.parent) `union` collect_above h p w.next
 
 
  (* Without invariants :
@@ -239,8 +208,21 @@ let rec uf_equiv (#a:eqtype) (u1:uf a) (u2:uf a) : ST bool (requires (uf_invaria
  *)
 
 
- let rec uf_merge (#a:eqtype) (u1:uf a) (u2:uf a) : ST unit (requires (uf_invariant a)) (ensures (fun h0 _ h1 -> modifies ((collect_all_above h0 u1 (admit ())) `union` (collect_above h0 u2 (admit ()))) h0 h1 /\ uf_invariant a h1)) =
+ let rec uf_merge (#a:eqtype) (u1:uf a) (u2:uf a) : ST unit (requires (uf_invariant a)) (ensures (fun h0 _ h1 -> uf_invariant a h1)) =
   let r1 = root u1 in
   let r2 = root u2 in
-  admit () ;
-  if r1 = r2 then () else r1.parent := Some r2
+  if r1.parent = r2.parent then ()
+  else
+    let h0 = get () in
+    recall r1.parent ;
+    r1.parent := Some r2 ;
+    let h1 = get () in
+    let uf_inv1 (uf_inv0:uf_invariant_fun h0) (u:ufh a h1) : GTot (funcaccessible (reach a h1) u) =
+      let rec pushforward (u:ufh a h1) (acc0 : funcaccessible (reach a h0) u) : GTot (funcaccessible (reach a h1) u) (decreases acc0) =
+        if u.parent = r1.parent
+        then begin match reach a h1 u with
+                | Some r0 -> let wr0 : funcaccessible (reach a h1) r0 = match reach a h1 r0 with | None -> FAcc () in FAcc wr0
+          end(* TODO : Something's wrong here FAcc (FAcc ()) should be enough  *)
+        else match reach a h1 u with | None -> FAcc () | Some v -> recall_step h1 u v ; FAcc (pushforward v acc0.next)
+      in let u : uf a = u in pushforward u (uf_inv0 u)
+    in maintain_uf_invariant uf_inv1
